## Problems

### 12-1 Binary search trees with equal keys

> Equal keys pose a problem for the implementation of binary search trees.

> __*a*__. What is the asymptotic performance of TREE-INSERT when used to insert $$n$$ items with identical keys into an initially empty binary search tree?

$$\Theta(n)$$

> __*b*__. Keep a boolean flag $$x.b$$ at node $$x$$, and set $$x$$ to either $$x.left$$ or $$x.right$$ based on the value of $$x.b$$, which alternates between FALSE and TRUE each time we visit $$x$$ while inserting a node with the same key as $$x$$.

$$\Theta(n \lg n)$$

> __*c*__. Keep a list of nodes with equal keys at $$x$$, and insert $$z$$ into the list.

If linked list is used, it could be $$\Theta(1)$$.

> __*d*__. Randomly set $$x$$ to either $$x.left$$ or $$x.right$$. (Give the worst-case performance and informally derive the expected running time.)

Worst: $$\Theta(n)$$.

Expected: $$\Theta(n \lg n)$$.

### 12-2 Radix trees

> Given two strings $$a = a_0a_1 \dots a_p$$ and $$b = b_0b_1 \dots b_q$$, where each $$a_i$$ and each $$b_j$$ is in some ordered set of characters, we say that string $$a$$ is lexicographically less
than string $$b$$ if either
1. there exists an integer $$j$$, where $$0 \le j \le \min(p, q)$$, such that $$a_i = b_i$$ for all $$i = 0, 1, \dots j - 1$$ and $$a_j < b_j$$, or
2. $$p < q$$ and $$a_i = b_i$$ for all $$i = 0, 1, \dots, p$$.

> The radix tree data structure shown in Figure 12.5 stores the bit strings 1011, 10, 011, 100, and 0. When searching for a key $$a = a_0a_1 \dots a_p$$, we go left at a node of depth $$i$$ if $$a_i = 0$$ and right if $$a_i = 1$$. Let $$S$$ be a set of distinct bit strings whose lengths sum to $$n$$. Show how to use a radix tree to sort $$S$$ lexicographically in $$\Theta(n)$$ time. For the example in Figure 12.5, the output of the sort should be the sequence 0, 011, 10, 100, 1011.

Insert all the bit strings into radix tree costs $$\Theta(n)$$, then use preorder tree walk to sort the strings costs $$\Theta(n)$$, the total cost is still $$\Theta(n)$$.

```python
class TreeNode:
    def __init__(self, val, left=None, right=None):
        self.val = val
        self.left = left
        self.right = right


class RadixTree:
    def __init__(self):
        self.root = None

    def insert(self, a):
        self.root = self.insert_rec(self.root, a, 0)

    def insert_rec(self, root, a, idx):
        if idx == len(a):
            if root is None:
                return TreeNode(a)
            root.val = a
            return root
        if root is None:
            root = TreeNode(None)
        if a[idx] == '0':
            root.left = self.insert_rec(root.left, a, idx+1)
        else:
            root.right = self.insert_rec(root.right, a, idx+1)
        return root

    def sorted(self):
        self.sorted_list = []
        self.sorted_rec(self.root)
        return self.sorted_list

    def sorted_rec(self, root):
        if root is None:
            return
        if root.val is not None:
            self.sorted_list.append(root.val)
        self.sorted_rec(root.left)
        self.sorted_rec(root.right)


def sort_strings(strs):
    radix_tree = RadixTree()
    for s in strs:
        radix_tree.insert(s)
    return radix_tree.sorted()
```

### 12-3 Average node depth in a randomly built binary search tree

> In this problem, we prove that the average depth of a node in a randomly built binary search tree with n nodes is $$O(\lg n)$$. Although this result is weaker than that of Theorem 12.4, the technique we shall use reveals a surprising similarity between the building of a binary search tree and the execution of RANDOMIZED-QUICKSORT from Section 7.3.

> We define the __*total path length*__ $$P(T)$$ of a binary tree $$T$$ as the sum, over all nodes $$x$$ in $$T$$ , of the depth of node $$x$$, which we denote by $$d(x, T)$$.

> __*a*__. Argue that the average depth of a node in $$T$$ is

> $$\displaystyle \frac{1}{n} \sum_{x \in T} d(x, T) = \frac{1}{n} P(T)$$.

Obviously.

> Thus, we wish to show that the expected value of $$P(T)$$ is $$O(n \lg n)$$.

> __*b*__. Let $$T_L$$ and $$T_R$$ denote the left and right subtrees of tree $$T$$, respectively. Argue that if $$T$$ has $$n$$ nodes, then

> $$P(T) = P(T_L) + P(T_R) + n - 1$$.

There are $$n-1$$ nodes in $$P(T_L)$$ and $$P(T_R)$$, each increase by 1.

> __*c*__. Let $$P(n)$$ denote the average total path length of a randomly built binary search tree with n nodes. Show that

> $$\displaystyle P(n) = \frac{1}{n} \sum_{i=0}^{n-1} (P(i) + P(n-i-1) + n - 1)$$.

The root is equally likely to be the rank in $$[1, n]$$.

> __*d*__. Show how to rewrite $$P(n)$$ as

> $$\displaystyle P(n) = \frac{2}{n} \sum_{k=1}^{n-1} P(k) + \Theta(n)$$.

Each item $$P(1), P(2), \dots, P(n)$$ appears twice in the summation, and

$$
\frac{1}{n} \sum_{i=0}^{n-1} n - 1 = \frac{(n-3)n}{2n} = \Theta(n)
$$

> __*e*__. Recalling the alternative analysis of the randomized version of quicksort given in Problem 7-3, conclude that $$P(n) = O(n \lg n)$$.

Based on Problem 7-3,  $$P(n) = O(n \lg n)$$.

> __*f*__. Describe an implementation of quicksort in which the comparisons to sort a set of elements are exactly the same as the comparisons to insert the elements into a binary search tree.

Choose the pivot that it has the lowest index in the original list.

### 12-4 Number of different binary trees

> Let $$b_n$$ denote the number of different binary trees with $$n$$ nodes. In this problem, you will find a formula for $$b_n$$, as well as an asymptotic estimate.

> __*a*__. Show that $$b_0 = 1$$ and that, for $$n \ge 1$$,

> $$\displaystyle b_n = \sum_{k=0}^{n-1} b_k b_{n-1-k}$$.

A root with two subtree.

> __*b*__. Referring to Problem 4-4 for the definition of a generating function, let $$B(x)$$ be the generating function

> $$\displaystyle B(x) = \sum_{n=0}^\infty b_n x^n$$.

$$
\begin{array}{rll}
B(x)^2 &=& (b_0 x^0 + b_1 x^1 + b_2 x^2 + \dots) ^ 2 \\
&=& b_0^2 x^0 + (b_0 b_1 + b_1 b_0) x^1 + (b_0 b_2 + b_1 b_1 + b_2 b_0) x^2 + \dots \\
&=& \displaystyle \sum_{k=0}^0 b_k b_{0-k} x^0 + \sum_{k=0}^1 b_k b_{1-k} x^1 + \sum_{k=0}^2 b_k b_{2-k} x^2 + \dots \\
\end{array}
$$

$$
\begin{array}{rll}
xB(x)^2 + 1 &=& \displaystyle 1 + \sum_{k=0}^0 b_k b_{1-1-k} x^1 + \sum_{k=0}^2 b_k b_{2-1-k} x^3 + \sum_{k=0}^2 b_k b_{3-1-k} x^2 + \dots \\
&=& 1 + b_1 x^1 + b_2 x^2 + b_3 x^3 + \dots \\
&=& b_0 x^0 + b_1 x^1 + b_2 x^2 + b_3 x^3 + \dots \\
&=& \displaystyle \sum_{n=0}^\infty b_n x^n \\
&=& B(x)
\end{array}
$$

> Show that $$B(x) = x B(x)^2 + 1$$, and hence one way to express $$B(x)$$ in closed form is

> $$\displaystyle B(x) = \frac{1}{2x} (1 - \sqrt{1 - 4x})$$.

$$
\begin{array}{rll}
x B(x)^2 + 1 &=& \displaystyle x \cdot \frac{1}{4x^2} (1 + 1 - 4x - 2\sqrt{1 - 4x}) + 1 \\
&=& \displaystyle \frac{1}{4x} (2 - 2\sqrt{1 - 4x}) - 1 + 1 \\
&=& \displaystyle \frac{1}{2x} (1 - \sqrt{1 - 4x}) \\
&=& B(x)
\end{array}
$$

> The __*Taylor expansion*__ of $$f(x)$$ around the point $$x=a$$ is given by

> $$\displaystyle f(x) = \sum_{k=0}^\infty \frac{f^{(k)}(a)}{k!} (x - a)^k$$,

> where $$f^{(k)}(a)$$ is the $$k$$th derivative of $$f$$ evaluated at $$x$$.

> __*c*__. Show that

> $$\displaystyle b_n = \frac{1}{n+1} \binom{2n}{n}$$

> (the $$n$$th Catalan number) by using the Taylor expansion of $$\sqrt{1-4x}$$ around $$x=0$$. 

Let $$f(x) = \sqrt{1-4x}$$,

The numerator of the derivative is 

$$\begin{array}{rll}
2 \cdot (1 \cdot 2) \cdot (3 \cdot 2) \cdot (5 \cdot 2)\cdots &=&
\displaystyle 2^k \cdot \prod_{i=0}^{k - 2}(2k+1) \\
&=& 2^k \cdot \frac{\displaystyle (2(k-1))!}{\displaystyle 2^{k-1}(k-1)!} \\
&=& \frac{\displaystyle 2(2(k-1))!}{\displaystyle (k-1)!} \\
\end{array}
$$

$$\displaystyle f(x) = 1 - 2x - 2x^2 - 4 x^3 - 10x^4 - 28x^5 - \dots$$

The coefficient is $$\frac{\displaystyle 2(2(k-1))!}{\displaystyle k!(k-1)!}$$.

$$\begin{array}{rll}
B(x) &=& \displaystyle \frac{1}{2x}(1-f(x)) \\
&=& 1 + x + 2x^2 + 5x^3 + 14x^4 + \dots \\
&=& \displaystyle \sum_{n=0}^\infty \frac{\displaystyle (2n)!}{\displaystyle (n+1)!n!} x \\
&=& \displaystyle \sum_{n=0}^\infty \frac{1}{n+1} \frac{\displaystyle (2n)!}{\displaystyle n!n!} x \\
&=& \displaystyle \sum_{n=0}^\infty \frac{1}{n+1} \binom{2n}{n} x
\end{array}
$$

Therefore $$\displaystyle b_n = \frac{1}{n+1} \binom{2n}{n}$$.

> __*d*__. Show that

> $$\displaystyle b_n = \frac{4^n}{\sqrt{\pi}n^{3/2}} (1 + O(1/n))$$.

Based on Stirling's approximation $$\displaystyle n! \approx \sqrt{2 \pi n} \left ( \frac{n}{e} \right )^n$$,

$$
\begin{array}{rll}
b_n &=& \displaystyle \frac{1}{n+1} \frac{\displaystyle (2n)!}{\displaystyle n!n!} \\
&\approx& \displaystyle \frac{1}{n+1} \frac{\sqrt{4 \pi n}(2n / e)^{2n}}{2 \pi n (n/e)^{2n}} \\
&=& \displaystyle \frac{1}{n+1} \frac{4^n}{\sqrt{\pi n} } \\
&=& \displaystyle \left ( \frac{1}{n} + \left ( \frac{1}{n+1} - \frac{1}{n} \right ) \right ) \frac{4^n}{\sqrt{\pi n} } \\
&=& \displaystyle \left ( \frac{1}{n} - \frac{1}{n^2+n} \right ) \frac{4^n}{\sqrt{\pi n} } \\
&=& \displaystyle \frac{1}{n} \left (1  - \frac{1}{n+1} \right ) \frac{4^n}{\sqrt{\pi n} } \\
&=& \displaystyle \frac{4^n}{\sqrt{\pi}n^{3/2}} (1 + O(1/n))
\end{array}
$$
